Add typing rules for maps
Updated logging2.v to include typechecking theorems, which all work now.

src/go_lang/map.v
@@ -1,6 +1,0 @@
-From Perennial.go_lang Require Export lang notation.
-From Perennial.go_lang Require Import typing.
-
-Definition NewMap {ext:ext_op} (t:ty) : expr := AllocMap (zero_val t).
-
-Definition mapT (vt:ty) : ty := refT (mapValT vt).
